finish up proofs, just have to fix framing with isplitl and bool_decide

src/Examples/DistributedCtr/DistCtrImpl.v
@@ -61,7 +61,7 @@ Definition update_replicas: val :=
   acquire "lk2";;
   let: "s1" := update_node "node1" in
   let: "s2" := update_node "node2" in
-  if: "s1" = #0 then
+  if: (("s1" = #0) || ("s2" = #0) then
     recover_replicas "node1" "node2";;
     release "lk2";;
     release "lk1"
@@ -452,10 +452,10 @@ Qed.
         iFrame; auto.
 
     - iDestruct "Honedead" as "[(Hnode1 & Hnode2) | (Hnode1 & Hnode2)]".
-      wp_apply (update_node_none_spec with "[Hnode1 Hown1 Hγ1●]").
-      unfold node_val_inv.
-      iFrame; auto.
-      iIntros "(Hnode1 & Hnodelkinv1 & Hvalinv1)". wp_let; wp_pures.
+      * wp_apply (update_node_none_spec with "[Hnode1 Hown1 Hγ1●]").
+        unfold node_val_inv.
+        iFrame; auto.
+        iIntros "(Hnode1 & Hnodelkinv1 & Hvalinv1)". wp_let; wp_pures.
 
         wp_apply (update_node_some_spec with "[Hnode2 Hown2 Hγ2●]").
         unfold node_val_inv.
@@ -465,8 +465,9 @@ Qed.
         wp_apply ((recover_replicas_one_dead_spec (n'+1) γ1 γ2)
                     with "[- HPost Hlked1 Hlked2 Hnodelkinv1 Hnodelkinv2]").
         iFrame; auto.
-        unfold global_inv. iFrame; auto.
-        admit. (* TODO how to deal with framing here? *)
+        unfold global_inv. iFrame; auto. iSplit; iFrame; auto.
+        admit. (* TODO bool_decide *)
+        admit. (* TODO framing  *)
 
         iIntros "(Hnval & Hnode1 & Hnode2 & Hinv)".
         wp_pures.
@@ -477,23 +478,87 @@ Qed.
         wp_apply (release_spec with "[Hlkinv1 Hnodelkinv1 Hlked1]"); iFrame; auto.
         iIntros; wp_pures.
         iApply "HPost"; iSplit; auto. iFrame; iSplit; auto.
-  Qed.
+
+      * wp_apply (update_node_some_spec with "[Hnode1 Hown1 Hγ1●]").
+        unfold node_val_inv.
+        iFrame; auto.
+        iIntros "(Hnode1 & Hnodelkinv1 & Hvalinv1)". wp_let; wp_pures.
+
+        wp_apply (update_node_none_spec with "[Hnode2 Hown2 Hγ2●]").
+        unfold node_val_inv.
+        iFrame; auto.
+        iIntros "(Hnode2 & Hnodelkinv2 & Hvalinv2)". wp_let; wp_pures.
+
+        wp_apply ((recover_replicas_one_dead_spec (n'+1) γ1 γ2)
+        with "[- HPost Hlked1 Hlked2 Hnodelkinv1 Hnodelkinv2]").
+        iFrame; auto.
+        unfold global_inv. iFrame; auto. iSplit; iFrame; auto.
+        admit. (* TODO bool_decide *)
+        admit. (* TODO framing  *)
+
+            iIntros "(Hnval & Hnode1 & Hnode2 & Hinv)".
+            wp_pures.
+
+            wp_apply (release_spec with "[Hlkinv2 Hlked2 Hnodelkinv2]"). iSplit; auto. iFrame; auto.
+            iIntros; wp_pures.
+
+            wp_apply (release_spec with "[Hlkinv1 Hnodelkinv1 Hlked1]"); iFrame; auto.
+            iIntros; wp_pures.
+            iApply "HPost"; iSplit; auto. iFrame. iSplit; auto.
+  Admitted.
 
   Lemma update_replicas_both_dead_spec : ∀ (n: Z) γ1 γ2 γ3 γ4 lk1 lk2 node1 node2,
       {{{
            (node1 ↦ NONEV ∗ node2 ↦ NONEV)
-           ∗ is_lock LockN γ3 lk1 (node_lock_inv n γ1)
-           ∗ is_lock LockN γ4 lk2 (node_lock_inv n γ2)
-           ∗ global_inv n (Some n) (Some n) γ1 γ2
+           ∗ is_lock LockN γ3 lk1 (node_lock_inv γ1)
+           ∗ is_lock LockN γ4 lk2 (node_lock_inv γ2)
+           ∗ global_inv (Some n) (Some n) γ1 γ2
     }}}
-      update_replicas #node1 lk1 #node2 lk2
+      update_replicas #node1 #node2 lk1 lk2
     {{{ RET #();
            node1 ↦ SOMEV #(0) ∗ node2 ↦ SOMEV #(0)
-           ∗ is_lock LockN γ3 lk1 (node_lock_inv (0) γ1)
-           ∗ is_lock LockN γ4 lk2 (node_lock_inv (0) γ2)
-           ∗ global_inv (0) (Some 0) (Some 0) γ1 γ2
+           ∗ is_lock LockN γ3 lk1 (node_lock_inv γ1)
+           ∗ is_lock LockN γ4 lk2 (node_lock_inv γ2)
+           ∗ global_inv (Some 0) (Some 0) γ1 γ2
     }}}.
   Proof.
-  Admitted.
+    iIntros (n γ1 γ2 γ3 γ4 lk1 lk2 node1 node2 ϕ) "((Hnode1 & Hnode2) & #Hlkinv1 & #Hlkinv2 & Hglobalinv) HPost".
+    unfold global_inv; unfold node_val_inv; unfold node_lock_inv.
+    iDestruct "Hglobalinv" as (n') "(Hown1 & Hown2)".
+    iDestruct "Hown1" as (Hn) "Hown1".
+    iDestruct "Hown2" as (_) "Hown2".
+    destruct Hn; inversion H; subst.
+    unfold update_replicas.
+    wp_pures.
+    wp_apply (acquire_spec with "Hlkinv1");
+      iIntros "(Hlked1 & Hγ1●)"; wp_pures;
+      wp_apply (acquire_spec with "Hlkinv2");
+      iIntros "(Hlked2 & Hγ2●)"; wp_pures.
+
+    wp_apply (update_node_none_spec with "[Hnode1 Hown1 Hγ1●]").
+        unfold node_val_inv.
+        iFrame; auto.
+        iIntros "(Hnode1 & Hnodelkinv1 & Hvalinv1)". wp_let; wp_pures.
+
+    wp_apply (update_node_none_spec with "[Hnode2 Hown2 Hγ2●]").
+        unfold node_val_inv.
+        iFrame; auto.
+        iIntros "(Hnode2 & Hnodelkinv2 & Hvalinv2)". wp_let; wp_pures.
+
+    wp_apply ((recover_replicas_both_dead_spec 0 γ1 γ2)
+                with "[- HPost Hlked1 Hlked2]"). 
+    iFrame; unfold global_inv; unfold node_lock_inv; unfold node_val_inv; auto.
+    iExists 0; iFrame; auto.
+
+    iIntros "(Hnode1 & Hnode2 & Hinv & Hn1inv & Hn2inv)".
+    wp_pures.
+    wp_apply (release_spec with "[Hlked2 Hlkinv2 Hn2inv]").
+    iFrame; auto.
+    iIntros; wp_pures.
+    wp_apply (release_spec with "[Hlked1 Hlkinv1 Hn1inv]").
+    iFrame; auto.
+    iIntros; wp_pures.
+    iApply "HPost". iFrame. iSplit; auto. 
+  Qed.
 
 End proof.
